Rm the modal separation

src/dynamics.lean
@@ -1,16 +1,21 @@
 import syntax
 
-inductive steps: cx val -> exp -> cx val -> exp -> Prop
+inductive val: exp -> Prop
+| int (n: ℤ): val (exp.int n)
+| true: val exp.true
+| false: val exp.false
+
+inductive steps: cx exp -> exp -> cx exp -> exp -> Prop
 | if_e1
-    (Δ: cx val) (Δ': cx val)
+    (Δ: cx exp) (Δ': cx exp)
     (e1: exp) (e1': exp) (e2: exp) (e3: exp):
     steps Δ e1 Δ' e1' ->
     steps Δ (exp.if_ e1 e2 e3) Δ' (exp.if_ e1' e2 e3)
 | if_true
-    (Δ: cx val)
+    (Δ: cx exp)
     (e2: exp) (e3: exp):
-    steps Δ (exp.if_ (exp.pure val.true) e2 e3) Δ e2
+    steps Δ (exp.if_ exp.true e2 e3) Δ e2
 | if_false
-    (Δ: cx val)
+    (Δ: cx exp)
     (e2: exp) (e3: exp):
-    steps Δ (exp.if_ (exp.pure val.false) e2 e3) Δ e3
+    steps Δ (exp.if_ exp.false e2 e3) Δ e3
