src/statics.lean
@@ -1,19 +1,13 @@
 import syntax
 
-inductive val_typ: cx typ -> val -> typ -> Prop
-| int (Γ: cx typ) (n: ℤ): val_typ Γ (val.int n) typ.int
-| true (Γ: cx typ): val_typ Γ val.true typ.bool
-| false (Γ: cx typ): val_typ Γ val.false typ.bool
-
-inductive exp_typ: cx typ -> exp -> typ -> Prop
-| pure
-    (Γ: cx typ) (v: val) (τ: typ):
-    val_typ Γ v τ ->
-    exp_typ Γ (exp.pure v) τ
+inductive has_typ: cx typ -> exp -> typ -> Prop
+| int (Γ: cx typ) (n: ℤ): has_typ Γ (exp.int n) typ.int
+| true (Γ: cx typ): has_typ Γ exp.true typ.bool
+| false (Γ: cx typ): has_typ Γ exp.false typ.bool
 | if_
     (Γ: cx typ)
     (e1: exp) (e2: exp) (e3: exp) (τ: typ):
-    exp_typ Γ e1 typ.bool ->
-    exp_typ Γ e2 τ ->
-    exp_typ Γ e3 τ ->
-    exp_typ Γ (exp.if_ e1 e2 e3) τ
+    has_typ Γ e1 typ.bool ->
+    has_typ Γ e2 τ ->
+    has_typ Γ e3 τ ->
+    has_typ Γ (exp.if_ e1 e2 e3) τ
