src/syntax.lean
@@ -4,11 +4,8 @@ inductive typ: Type
 | int: typ
 | bool: typ
 
-inductive val: Type
-| int: ℤ -> val
-| true: val
-| false: val
-
 inductive exp: Type
-| pure: val -> exp
+| int: ℤ -> exp
+| true: exp
+| false: exp
 | if_: exp -> exp -> exp -> exp
