src/safety.lean
@@ -1,26 +1,28 @@
 import helpers
 
 theorem progress
-  (Γ: cx typ) (Δ: cx val)
+  (Γ: cx typ) (Δ: cx exp)
   (tcx_nil: Γ = list.nil)
   (vcx_nil: Δ = list.nil)
   (e: exp) (τ: typ)
-  (et: exp_typ Γ e τ)
-  : (∃ (v: val), e = exp.pure v) ∨ (∃ (Δ': cx val) (e': exp), steps Δ e Δ' e') :=
+  (et: has_typ Γ e τ)
+  : val e ∨ (∃ (Δ': cx exp) (e': exp), steps Δ e Δ' e') :=
 begin
   induction et,
   left,
-  existsi et_v,
-  refl,
+  exact val.int et_n,
+  left,
+  exact val.true,
+  left,
+  exact val.false,
   right,
   cases et_ih_a tcx_nil,
-  cases h,
-  rewrite h_h at *,
-  cases bool_canonical_forms et_Γ h_w (inversion_pure et_Γ h_w typ.bool et_a),
-  rewrite h,
+  -- rewrite h_h at *,
+  cases bool_canonical_forms et_Γ et_e1 h et_a,
+  rewrite h_1,
   existsi [Δ, et_e2],
   exact steps.if_true Δ et_e2 et_e3,
-  rewrite h,
+  rewrite h_1,
   existsi [Δ, et_e3],
   exact steps.if_false Δ et_e2 et_e3,
   cases h,
@@ -30,20 +32,20 @@ begin
 end
 
 theorem preservation
-  (Γ: cx typ) (Δ: cx val) (Δ': cx val)
+  (Γ: cx typ) (Δ: cx exp) (Δ': cx exp)
   (tcx_nil: Γ = list.nil)
   (vcx_nil: Δ = list.nil)
   (e: exp) (e': exp) (τ: typ)
-  (et: exp_typ Γ e τ)
+  (et: has_typ Γ e τ)
   (st: steps Δ e Δ' e')
-  : exp_typ Γ e' τ :=
+  : has_typ Γ e' τ :=
 begin
   induction st generalizing Γ τ,
   let inv := inversion_if Γ st_e1 st_e2 st_e3 τ et,
   let e1_typ := st_ih vcx_nil Γ typ.bool tcx_nil inv.left,
-  exact exp_typ.if_ Γ st_e1' st_e2 st_e3 τ e1_typ inv.right.left inv.right.right,
-  let inv := inversion_if Γ (exp.pure val.true) st_e2 st_e3 τ et,
+  exact has_typ.if_ Γ st_e1' st_e2 st_e3 τ e1_typ inv.right.left inv.right.right,
+  let inv := inversion_if Γ exp.true st_e2 st_e3 τ et,
   exact inv.right.left,
-  let inv := inversion_if Γ (exp.pure val.false) st_e2 st_e3 τ et,
+  let inv := inversion_if Γ exp.false st_e2 st_e3 τ et,
   exact inv.right.right,
 end
